FokkerChallenge.lean
@@ -17,6 +17,7 @@ import FokkerChallenge.EnhancedCslib.LeftMost
 import FokkerChallenge.EnhancedCslib.Closedunderapp
 import FokkerChallenge.EnhancedCslib.FlipApp
 import FokkerChallenge.EnhancedCslib.List
+import FokkerChallenge.EnhancedCslib.Spine
 import FokkerChallenge.Decider.NoDuplicate
 import FokkerChallenge.Decider.EveryBvarUsed
 import FokkerChallenge.Decider.All0
