FokkerChallenge/EnhancedCslib/Spine.lean
@@ -1,0 +1,16 @@
+import Cslib.Languages.LambdaCalculus.LocallyNameless.Untyped.Basic
+
+namespace Cslib
+
+namespace LambdaCalculus.LocallyNameless.Untyped.Term
+
+@[scoped grind]
+def spine : Term String → Term String × List (Term String)
+  | Term.app f a => let (h, args) := spine f; (h, args ++ [a])
+  | t            => (t, [])
+
+theorem spine_def {t l f} : spine t = (f, l) -> l.foldl Term.app f = t := by
+  induction t generalizing l f with grind
+
+theorem spine_def_2 (t : Term String) : t.spine.2.foldl Term.app t.spine.1 = t := by
+  induction t with grind
